implement transition from F_HANDSHAKE_B -> F_SYNC

ironfleet/src/Dafny/Distributed/Protocol/ZooKeeper/Follower.dfy
@@ -13,10 +13,11 @@ datatype Follower = Follower(
     leader_id: nat,
     config: Config,
     zkdb: ZKDatabase,
+    accepted_epoch: int,
     state: FollowerState 
 )
 
-datatype FollowerState = F_HANDSHAKE_A | F_HANDSHAKE_B | F_SYNC | F_RUNNING
+datatype FollowerState = F_HANDSHAKE_A | F_HANDSHAKE_B | F_SYNC | F_RUNNING | F_ERROR
 
 predicate FollowerInit(s:Follower, my_id:nat, leader_id:nat, config:Config, zkdb: ZKDatabase)
 {
@@ -24,6 +25,7 @@ predicate FollowerInit(s:Follower, my_id:nat, leader_id:nat, config:Config, zkdb
     && s.leader_id == leader_id
     && s.config == config
     && s.zkdb == zkdb
+    && s.accepted_epoch == -1
     && s.state == F_HANDSHAKE_A
 }
 
@@ -33,6 +35,7 @@ predicate FollowerNext(s:Follower, s':Follower, ios:seq<ZKIo>) {
         case F_HANDSHAKE_B => false // TODO
         case F_SYNC => false  // TODO
         case F_RUNNING => false  // TODO
+        case F_ERROR => s' == s  // TODO
 }
 
 
@@ -49,5 +52,34 @@ predicate SendMyInfo(s:Follower, s':Follower, ios:seq<ZKIo>) {
         && if |s.zkdb.commitLog| == 0 
             then outbound_packet.msg.latestZxid == NullZxid
             else outbound_packet.msg.latestZxid == s.zkdb.commitLog[|s.zkdb.commitLog|-1]
+}
+
+
+/* State transition from F_HANDSHAKE_B -> F_SYNC */
+predicate AcceptNewEpoch(s:Follower, s':Follower, ios:seq<ZKIo>) {
+    // state and epoch are the only properties that change in this transition
+    && s' == s.(state := s'.state, accepted_epoch := s'.accepted_epoch)  
+    && |ios| >= 1
+    && 0 <= s.leader_id < |s.config|
+    && ios[0].LIoOpReceive?
+    && ios[0].r.msg.LeaderInfo?
+    && ios[0].r.msg.sid == s.leader_id
+    && (if ios[0].r.msg.newZxid.epoch <  s.accepted_epoch 
+        then && s'.state == F_ERROR
+             && |ios| == 1
+        else (
+            && s'.state == F_SYNC
+            && s'.accepted_epoch == ios[0].r.msg.newZxid.epoch
+            && |ios| == 2
+            && ios[1].LIoOpSend?
+            && ios[1].s.dst == s.config[s.leader_id]
+            && ios[1].s.msg.AckEpoch?
+            && ios[1].s.msg.sid == s.my_id
+            && ios[1].s.msg.lastLoggedZxid == getLastLoggedZxid(s.zkdb)
+            && if ios[0].r.msg.newZxid.epoch ==  s.accepted_epoch
+                then ios[1].s.msg.lastAcceptedEpoch == -1
+                else ios[1].s.msg.lastAcceptedEpoch == ios[0].r.msg.newZxid.epoch
+        )
+    )
 }
 }
