ironfleet/src/Dafny/Distributed/Protocol/ZooKeeper/Types.dfy
@@ -13,7 +13,10 @@ datatype EndPoint = EndPoint(addr:seq<byte>, port:uint16)
 
 type Config = seq<EndPoint>
 
-datatype ZKMessage = FollowerInfo(sid:nat, latestZxid:Zxid)
+datatype ZKMessage = 
+    | FollowerInfo(sid:nat, latestZxid:Zxid)
+    | LeaderInfo(sid:nat, newZxid:Zxid)
+    | AckEpoch(sid:nat, lastLoggedZxid:Zxid, lastAcceptedEpoch:int)
 
 type ZKEnvironment = LEnvironment<EndPoint, ZKMessage>
 type ZKPacket = LPacket<EndPoint, ZKMessage>
